Revert "Split things out into modules"
This reverts commit fe257c2a3f161dc4e708cf2a294b4d97d42ad5d5.

src/Parsers/BooleanRecognizer.v
@@ -1,357 +1,394 @@
 (** * Definition of a boolean-returning CFG parser-recognizer *)
 Require Import Omega.
-Require Import Coq.Lists.List Coq.Program.Program Coq.Program.Wf Coq.Arith.Wf_nat Coq.Arith.Compare_dec Coq.Classes.RelationClasses Coq.Strings.String Coq.Structures.Equalities.
-Require Import Parsers.ContextFreeGrammar Parsers.Specification Parsers.ListLike Parsers.ListListLike Parsers.StringStringLike.
+Require Import Coq.Lists.List Coq.Program.Program Coq.Program.Wf Coq.Arith.Wf_nat Coq.Arith.Compare_dec Coq.Classes.RelationClasses Coq.Strings.String.
+Require Import Parsers.ContextFreeGrammar Parsers.Specification.
 Require Import Common Common.ilist Common.Wf.
 
 Set Implicit Arguments.
+Local Open Scope string_like_scope.
 
-Module RecursiveDescentBooleanParserHelper (S : StringLike).
-  Import S.
-  Module Export CFG := ContextFreeGrammar S.
-  Module Productions <: Typ.
-    Definition t := productions.
-  End Productions.
+(** TODO: move this elsewhere *)
+Section recursive_descent_parser.
+  Context CharType (String : string_like CharType) (G : grammar CharType).
+  Context (productions_listT : Type)
+          (initial_productions_data : productions_listT)
+          (is_valid_productions : productions_listT -> productions CharType -> bool)
+          (remove_productions : productions_listT -> productions CharType -> productions_listT)
+          (productions_listT_R : productions_listT -> productions_listT -> Prop)
+          (remove_productions_dec : forall ls prods, is_valid_productions ls prods = true
+                                                     -> productions_listT_R (remove_productions ls prods) ls)
+          (ntl_wf : well_founded productions_listT_R).
+  Section bool.
+    Context (split_string_for_production
+             : forall (str0 : String) (prod : production CharType), list (String * String))
+            (split_string_for_production_correct
+             : forall str0 prod,
+                 List.Forall (fun s1s2 => (fst s1s2 ++ snd s1s2 =s str0) = true)
+                             (split_string_for_production str0 prod)).
 
-  Module RecursiveDescentBooleanParser (Listish : ListLike Productions).
-    Export Listish.
-    Local Open Scope list_like_scope.
-    Local Open Scope string_like_scope.
-    Local Notation String := S.t.
-    Local Notation productions_listT := Listish.t.
-    Local Notation remove_productions_dec := Listish.lt_1.
-    Section recursive_descent_parser.
-      Context (G : grammar).
-      Context (initial_productions_data : productions_listT).
-
-      Section bool.
-        Context (split_string_for_production
-                 : forall (str0 : String) (prod : production), list (String * String))
-                (split_string_for_production_correct
-                 : forall str0 prod,
-                     List.Forall (fun s1s2 => (fst s1s2 ++ snd s1s2 =s str0) = true)
-                                 (split_string_for_production str0 prod)).
-
-        Section parts.
-          Section item.
-            (** We require that the list of productions be non-empty; we
+    Section parts.
+      Section item.
+        (** We require that the list of productions be non-empty; we
             do this by passing the first element separately, rather
             than invoking dependent types and proofs. *)
-            Context (str : String)
-                    (str_matches_productions : production -> productions -> bool).
+        Context (str : String)
+                (str_matches_productions : production CharType -> productions CharType -> bool).
 
-            Definition parse_item (it : item) : bool
-              := match it with
-                   | Terminal ch => [[ ch ]] =s str
-                   | NonTerminal name => match Lookup G name with
-                                           | nil => (** No string can match an empty nonterminal *) false
-                                           | p::ps => str_matches_productions p ps
-                                         end
-                 end.
-          End item.
+        Definition parse_item (it : item CharType) : bool
+          := match it with
+               | Terminal ch => [[ ch ]] =s str
+               | NonTerminal name => match Lookup G name with
+                                       | nil => (** No string can match an empty nonterminal *) false
+                                       | p::ps => str_matches_productions p ps
+                                     end
+             end.
+      End item.
 
-          Section production.
-            Variable str0 : String.
-            Variable parse_productions : forall (str : String),
-                                           str ≤s str0
-                                           -> production
-                                           -> productions
-                                           -> bool.
+      Section production.
+        Variable str0 : String.
+        Variable parse_productions : forall (str : String),
+                                       str ≤s str0
+                                       -> production CharType
+                                       -> productions CharType
+                                       -> bool.
 
-            (** To match a [production], we must match all of its items.
+        (** To match a [production], we must match all of its items.
             But we may do so on any particular split. *)
-            Fixpoint parse_production
-                     (str : String) (pf : str ≤s str0)
-                     (prod : production)
-            : bool.
-            Proof.
-              refine match prod with
-                       | nil =>
-                         (** 0-length production, only accept empty *)
-                         str =s Empty
-                       | it::its
-                         => let parse_production' := fun str pf => @parse_production str pf its in
-                            fold_right
-                              orb
-                              false
-                              (map (fun s1s2p => (parse_item (fst (proj1_sig s1s2p))
-                                                             (@parse_productions (fst (proj1_sig s1s2p))
-                                                                                 _)
-                                                             it)
-                                                   && parse_production' (snd (proj1_sig s1s2p)) _)%bool
-                                   (combine_sig (split_string_for_production_correct str prod)))
-                     end;
-              revert pf; clear; intros;
-              abstract (
-                  repeat first [ progress destruct_head sig
-                               | progress destruct_head and
-                               | etransitivity; eassumption
-                               | etransitivity; try eassumption; []
-                               | progress subst
-                               | idtac; match goal with H : (_ =s _) = true |- _ => apply bool_eq_correct in H end
-                               | apply str_le1_append
-                               | apply str_le2_append ]
-                ).
-            Defined.
-          End production.
+        Fixpoint parse_production
+                 (str : String) (pf : str ≤s str0)
+                 (prod : production CharType)
+        : bool.
+        Proof.
+          refine match prod with
+                   | nil =>
+                     (** 0-length production, only accept empty *)
+                     str =s Empty _
+                   | it::its
+                     => let parse_production' := fun str pf => @parse_production str pf its in
+                        fold_right
+                          orb
+                          false
+                          (map (fun s1s2p => (parse_item (fst (proj1_sig s1s2p))
+                                                         (@parse_productions (fst (proj1_sig s1s2p))
+                                                                             _)
+                                                         it)
+                                               && parse_production' (snd (proj1_sig s1s2p)) _)%bool
+                               (combine_sig (split_string_for_production_correct str prod)))
+                 end;
+          revert pf; clear; intros;
+          abstract (
+              repeat first [ progress destruct_head sig
+                           | progress destruct_head and
+                           | etransitivity; eassumption
+                           | etransitivity; try eassumption; []
+                           | progress subst
+                           | idtac; match goal with H : (_ =s _) = true |- _ => apply bool_eq_correct in H end
+                           | apply str_le1_append
+                           | apply str_le2_append ]
+            ).
+        Defined.
+      End production.
 
-          Section productions.
-            Section step.
-              Variable str0 : String.
-              Variable parse_productions : forall (str : String)
-                                                  (pf : str ≤s str0),
-                                             production -> productions -> bool.
+      Section productions.
+        Section step.
+          Variable str0 : String.
+          Variable parse_productions : forall (str : String)
+                                              (pf : str ≤s str0),
+                                         production CharType -> productions CharType -> bool.
 
-              (** To parse as a given list of [production]s, we must parse as one of the [production]s. *)
-              Definition parse_productions_step (str : String) (pf : str ≤s str0) (prods : productions)
-              : bool
-                := fold_right orb
-                              false
-                              (map (parse_production parse_productions pf)
-                                   prods).
-            End step.
+          (** To parse as a given list of [production]s, we must parse as one of the [production]s. *)
+          Definition parse_productions_step (str : String) (pf : str ≤s str0) (prods : productions CharType)
+          : bool
+            := fold_right orb
+                          false
+                          (map (parse_production parse_productions pf)
+                               prods).
+        End step.
 
-            Section wf.
-              (** TODO: add comment explaining signature *)
-              Definition parse_productions_or_abort_helper
-              : forall (p : String * productions_listT) (str : String),
-                  str ≤s fst p
-                  -> production
-                  -> productions
-                  -> bool.
-              Proof.
-                refine (@Fix4
-                          (prod String productions_listT) _ _ _ _
-                          _ (@well_founded_prod_relation
-                               String
-                               productions_listT
-                               _
-                               _
-                               (well_founded_ltof _ Length)
-                               Listish.lt_wf)
-                          _ _).
-                refine (fun sl parse_productions str pf (prod : production) (prods : productions)
-                        => let str0 := fst sl in
-                           let valid_list := snd sl in
-                           match lt_dec (Length str) (Length str0) with
-                             | left pf' =>
-                               (** [str] got smaller, so we reset the valid productions list *)
-                               parse_productions_step
-                                 (parse_productions
-                                    (str, initial_productions_data)
-                                    (or_introl pf'))
-                                 (reflexivity _)
-                                 (prod::prods)
-                             | right pf' =>
-                               (** [str] didn't get smaller, so we cache the fact that we've hit this productions already *)
-                               (if (prod::prods) ∈ valid_list as is_valid
-                                   return (prod::prods) ∈ valid_list = is_valid -> _
-                                then (** It was valid, so we can remove it *)
-                                  fun H' =>
-                                    parse_productions_step
-                                      (parse_productions
-                                         (str0, remove (prod::prods) valid_list)
-                                         (or_intror (conj eq_refl (remove_productions_dec H'))))
-                                      (reflexivity _)
-                                      (prod::prods)
-                                else (** oops, we already saw this productions in the past.  ABORT! *)
-                                  fun _ => false
-                               ) eq_refl
-                           end).
-              Defined.
+        Section wf.
+          (** TODO: add comment explaining signature *)
+          Definition parse_productions_or_abort_helper
+          : forall (p : String * productions_listT) (str : String),
+              str ≤s fst p
+              -> production CharType
+              -> productions CharType
+              -> bool
+            := @Fix4
+                 (prod String productions_listT) _ _ _ _
+                 _ (@well_founded_prod_relation
+                      String
+                      productions_listT
+                      _
+                      _
+                      (well_founded_ltof _ Length)
+                      ntl_wf)
+                 _
+                 (fun sl parse_productions str pf (prod : production CharType) (prods : productions CharType)
+                  => let str0 := fst sl in
+                     let valid_list := snd sl in
+                     match lt_dec (Length str) (Length str0) with
+                       | left pf' =>
+                         (** [str] got smaller, so we reset the valid productions list *)
+                         parse_productions_step
+                           (parse_productions
+                              (str, initial_productions_data)
+                              (or_introl pf'))
+                           (or_intror eq_refl)
+                           (prod::prods)
+                       | right pf' =>
+                         (** [str] didn't get smaller, so we cache the fact that we've hit this productions already *)
+                         (if is_valid_productions valid_list (prod::prods) as is_valid
+                             return is_valid_productions valid_list (prod::prods) = is_valid -> _
+                          then (** It was valid, so we can remove it *)
+                            fun H' =>
+                              parse_productions_step
+                                (parse_productions
+                                   (str0, remove_productions valid_list (prod::prods))
+                                   (or_intror (conj eq_refl (remove_productions_dec H'))))
+                                (or_intror eq_refl)
+                                (prod::prods)
+                          else (** oops, we already saw this productions in the past.  ABORT! *)
+                            fun _ => false
+                         ) eq_refl
+                     end).
 
-              Definition parse_productions_or_abort (str0 str : String)
-                         (valid_list : productions_listT)
-                         (pf : str ≤s str0)
-                         (prods : productions)
-              : bool
-                := match prods with
-                     | nil => false
-                     | p::ps => parse_productions_or_abort_helper (str0, valid_list) pf p ps
-                   end.
+          Definition parse_productions_or_abort (str0 str : String)
+                     (valid_list : productions_listT)
+                     (pf : str ≤s str0)
+                     (prods : productions CharType)
+          : bool
+            := match prods with
+                 | nil => false
+                 | p::ps => parse_productions_or_abort_helper (str0, valid_list) pf p ps
+               end.
 
-              Definition parse_productions (str : String) (prods : productions)
-              : bool
-                := @parse_productions_or_abort str str initial_productions_data
-                                               (reflexivity _) prods.
-            End wf.
-          End productions.
-        End parts.
-      End bool.
-    End recursive_descent_parser.
-  End RecursiveDescentBooleanParser.
-End RecursiveDescentBooleanParserHelper.
+          Definition parse_productions (str : String) (prods : productions CharType)
+          : bool
+            := @parse_productions_or_abort str str initial_productions_data
+                                           (or_intror eq_refl) prods.
+        End wf.
+      End productions.
+    End parts.
+  End bool.
+End recursive_descent_parser.
 
-Module Export RecursiveDescentBooleanParserWithStringListHelper.
-  Module Import RecursiveDescentBooleanParserWithStringListHelper' := RecursiveDescentBooleanParserHelper StringStringLike.
-  Import CFG.
-  Module ProductionsDec <: EqDecType.
-    Include Productions.
-    Definition eqb (x y : t) : bool
-      := if productions_dec Ascii.ascii_dec x y then true else false.
-    Lemma eqb_1 : forall x, eqb x x = true.
-    Proof. unfold eqb; intros; edestruct productions_dec; congruence. Qed.
-    Lemma eqb_2 : forall x y, eqb x y = true -> x = y.
-    Proof. unfold eqb; intros; edestruct productions_dec; congruence. Qed.
-  End ProductionsDec.
-  Module L := ListListLike ProductionsDec.
-  Local Open Scope list_like_scope.
-  Local Open Scope string_like_scope.
-  Import StringStringLike.
-  Local Notation String := StringStringLike.t.
-  Local Notation productions_listT := L.t.
-  Local Notation remove_productions_dec := L.lt_1.
-  Module Import RecursiveDescentBooleanParserWithStringList := RecursiveDescentBooleanParser L.
-  (** TODO: move this elsewhere *)
-  Section example_parse_string_grammar.
-    Fixpoint make_all_single_splits (str : string) : list (string * string)
-      := ((""%string, str))
-           ::(match str with
-                | ""%string => nil
-                | String.String ch str' =>
-                  map (fun p => (String.String ch (fst p), snd p))
-                      (make_all_single_splits str')
-              end).
+Section recursive_descent_parser_list.
+  Context {CharType} {String : string_like CharType} {G : grammar CharType}.
+  Variable (CharType_eq_dec : forall x y : CharType, {x = y} + {x <> y}).
+  Definition rdp_list_productions_listT : Type := list (productions CharType).
+  Definition rdp_list_is_valid_productions : rdp_list_productions_listT -> productions CharType -> bool
+    := fun ls nt => if in_dec (productions_dec CharType_eq_dec) nt ls then true else false.
+  Definition rdp_list_remove_productions : rdp_list_productions_listT -> productions CharType -> rdp_list_productions_listT
+    := fun ls nt =>
+         filter (fun x => if productions_dec CharType_eq_dec nt x then false else true) ls.
+  Definition rdp_list_productions_listT_R : rdp_list_productions_listT -> rdp_list_productions_listT -> Prop
+    := ltof _ (@List.length _).
+  Lemma filter_list_dec {T} f (ls : list T) : List.length (filter f ls) <= List.length ls.
+  Proof.
+    induction ls; trivial; simpl in *.
+    repeat match goal with
+             | [ |- context[if ?a then _ else _] ] => destruct a; simpl in *
+             | [ |- S _ <= S _ ] => solve [ apply Le.le_n_S; auto ]
+             | [ |- _ <= S _ ] => solve [ apply le_S; auto ]
+           end.
+  Qed.
+  Lemma rdp_list_remove_productions_dec : forall ls prods,
+                                            @rdp_list_is_valid_productions ls prods = true
+                                            -> @rdp_list_productions_listT_R (@rdp_list_remove_productions ls prods) ls.
+  Proof.
+    intros.
+    unfold rdp_list_is_valid_productions, rdp_list_productions_listT_R, rdp_list_remove_productions, ltof in *.
+    destruct (in_dec (productions_dec CharType_eq_dec) prods ls); [ | discriminate ].
+    match goal with
+      | [ H : In ?prods ?ls |- context[filter ?f ?ls] ]
+        => assert (~In prods (filter f ls))
+    end.
+    { intro H'.
+      apply filter_In in H'.
+      destruct H' as [? H'].
+      destruct (productions_dec CharType_eq_dec prods prods); congruence. }
+    { match goal with
+        | [ |- context[filter ?f ?ls] ] => generalize dependent f; intros
+      end.
+      induction ls; simpl in *; try congruence.
+      repeat match goal with
+               | [ |- context[if ?x then _ else _] ] => destruct x; simpl in *
+               | [ H : _ \/ _ |- _ ] => destruct H
+               | _ => progress subst
+               | [ H : ~(_ \/ _) |- _ ] => apply Decidable.not_or in H
+               | [ H : _ /\ _ |- _ ] => destruct H
+               | [ H : ?x <> ?x |- _ ] => exfalso; apply (H eq_refl)
+               | _ => apply Lt.lt_n_S
+               | _ => apply Le.le_n_S
+               | _ => apply filter_list_dec
+               | [ H : _ -> _ -> ?G |- ?G ] => apply H; auto
+             end. }
+  Qed.
+  Lemma rdp_list_ntl_wf : well_founded rdp_list_productions_listT_R.
+  Proof.
+    unfold rdp_list_productions_listT_R.
+    intro.
+    apply well_founded_ltof.
+  Defined.
+End recursive_descent_parser_list.
 
-    Lemma make_all_single_splits_correct_eq str
-    : List.Forall (fun strs => fst strs ++ snd strs = str)%string (make_all_single_splits str).
-    Proof.
-      induction str; simpl; constructor; auto.
-      apply Forall_map.
+(** TODO: move this elsewhere *)
+Section example_parse_string_grammar.
+  Fixpoint make_all_single_splits (str : string) : list (string * string)
+    := ((""%string, str))
+         ::(match str with
+              | ""%string => nil
+              | String.String ch str' =>
+                map (fun p => (String.String ch (fst p), snd p))
+                    (make_all_single_splits str')
+            end).
+
+  Lemma make_all_single_splits_correct_eq str
+  : List.Forall (fun strs => fst strs ++ snd strs = str)%string (make_all_single_splits str).
+  Proof.
+    induction str; simpl; constructor; auto.
+    apply Forall_map.
+    unfold compose; simpl.
+    revert IHstr; apply Forall_impl; intros.
+    subst; trivial.
+  Qed.
+
+  Local Opaque string_dec.
+  Lemma make_all_single_splits_correct_seq str
+  : List.Forall (fun strs : string_stringlike * string_stringlike
+                 => (fst strs ++ snd strs =s str) = true)%string_like (make_all_single_splits str).
+  Proof.
+    induction str; simpl; constructor; simpl; auto.
+    { rewrite string_dec_refl; reflexivity. }
+    { apply Forall_map.
       unfold compose; simpl.
       revert IHstr; apply Forall_impl; intros.
-      subst; trivial.
-    Qed.
+      match goal with H : (_ =s _) = true |- _ => apply bool_eq_correct in H end.
+      subst; rewrite string_dec_refl; reflexivity. }
+  Qed.
 
-    Local Opaque string_dec.
-    Lemma make_all_single_splits_correct_seq str
-    : List.Forall (fun strs : String * String
-                   => (fst strs ++ snd strs =s str))%string_like (make_all_single_splits str).
-    Proof.
-      induction str; unfold is_true in *; simpl; constructor; simpl; auto.
-      { unfold "=s"; rewrite string_dec_refl; reflexivity. }
-      { apply Forall_map.
-        unfold compose; simpl.
-        revert IHstr; apply Forall_impl; intros.
-        match goal with H : (_ =s _) = true |- _ => apply bool_eq_correct in H end.
-        subst; unfold "=s"; rewrite string_dec_refl; reflexivity. }
-    Qed.
+  Lemma make_all_single_splits_correct_str_le (str : string_stringlike)
+  : List.Forall (fun strs => fst strs ≤s str /\ snd strs ≤s str)%string (make_all_single_splits str).
+  Proof.
+    generalize (make_all_single_splits_correct_eq str).
+    apply Forall_impl.
+    intros; subst; split;
+    first [ apply str_le1_append
+          | apply str_le2_append ].
+  Qed.
 
-    Lemma make_all_single_splits_correct_str_le (str : String)
-    : List.Forall (fun strs => fst strs ≤s str /\ snd strs ≤s str)%string (make_all_single_splits str).
-    Proof.
-      generalize (make_all_single_splits_correct_eq str).
-      apply Forall_impl.
-      intros; subst; split;
-      first [ apply str_le1_append
-            | apply str_le2_append ].
-    Qed.
+  Local Hint Resolve NPeano.Nat.lt_lt_add_l NPeano.Nat.lt_lt_add_r NPeano.Nat.lt_add_pos_r NPeano.Nat.lt_add_pos_l : arith.
+  Local Hint Resolve str_le1_append str_le2_append.
 
-    Local Hint Resolve NPeano.Nat.lt_lt_add_l NPeano.Nat.lt_lt_add_r NPeano.Nat.lt_add_pos_r NPeano.Nat.lt_add_pos_l : arith.
-    Local Hint Resolve str_le1_append str_le2_append.
+  Variable G : grammar Ascii.ascii.
 
-    Variable G : grammar.
+  Definition brute_force_make_parse_of : @String Ascii.ascii string_stringlike
+                                         -> productions Ascii.ascii
+                                         -> bool
+    := @parse_productions
+         _
+         _
+         G
+         _
+         (Valid_nonterminals G)
+         (rdp_list_is_valid_productions Ascii.ascii_dec)
+         (rdp_list_remove_productions Ascii.ascii_dec)
+         _
+         (rdp_list_remove_productions_dec Ascii.ascii_dec) rdp_list_ntl_wf
+         (fun (str : string_stringlike) _ => make_all_single_splits str)
+         (fun str0 _ => make_all_single_splits_correct_seq str0).
+End example_parse_string_grammar.
 
-    Definition brute_force_make_parse_of : String
-                                           -> productions
-                                           -> bool
-      := @parse_productions
-           G
-           (Valid_nonterminals G)
-           (fun (str : String) _ => make_all_single_splits str)
-           (fun str0 _ => make_all_single_splits_correct_seq str0).
-  End example_parse_string_grammar.
+Module example_parse_empty_grammar.
+  Definition make_parse_of : forall (str : string)
+                                    (prods : productions Ascii.ascii),
+                               bool
+    := @brute_force_make_parse_of (trivial_grammar _).
 
-  Module example_parse_empty_grammar.
+
+
+  Definition parse : string -> bool
+    := fun str => make_parse_of str (trivial_grammar _).
+
+  Time Compute parse "".
+  Check eq_refl : true = parse "".
+  Time Compute parse "a".
+  Check eq_refl : false = parse "a".
+  Time Compute parse "aa".
+  Check eq_refl : false = parse "aa".
+End example_parse_empty_grammar.
+
+Section examples.
+  Section ab_star.
+
+    Fixpoint production_of_string (s : string) : production Ascii.ascii
+      := match s with
+           | EmptyString => nil
+           | String.String ch s' => (Terminal ch)::production_of_string s'
+         end.
+
+    Coercion production_of_string : string >-> production.
+
+    Fixpoint list_to_productions {T} (default : T) (ls : list (string * T)) : string -> T
+      := match ls with
+           | nil => fun _ => default
+           | (str, t)::ls' => fun s => if string_dec str s
+                                       then t
+                                       else list_to_productions default ls' s
+         end.
+
+    Delimit Scope item_scope with item.
+    Bind Scope item_scope with item.
+    Delimit Scope production_scope with production.
+    Delimit Scope production_assignment_scope with prod_assignment.
+    Bind Scope production_scope with production.
+    Delimit Scope productions_scope with productions.
+    Delimit Scope productions_assignment_scope with prods_assignment.
+    Bind Scope productions_scope with productions.
+    Notation "n0 ::== r0" := ((n0 : string)%string, (r0 : productions _)%productions) (at level 100) : production_assignment_scope.
+    Notation "[[[ x ;; .. ;; y ]]]" :=
+      (list_to_productions (nil::nil) (cons x%prod_assignment .. (cons y%prod_assignment nil) .. )) : productions_assignment_scope.
+
+    Local Open Scope string_scope.
+    Notation "<< x | .. | y >>" :=
+      (@cons (production _) (x)%production .. (@cons (production _) (y)%production nil) .. ) : productions_scope.
+
+    Notation "$< x $ .. $ y >$" := (cons (NonTerminal _ x) .. (cons (NonTerminal _ y) nil) .. ) : production_scope.
+
+    Definition ab_star_grammar : grammar Ascii.ascii :=
+      {| Start_symbol := "ab_star";
+         Lookup := [[[ ("" ::== (<< "" >>)) ;;
+                       ("ab" ::== << "ab" >>) ;;
+                       ("ab_star" ::== << $< "" >$
+                                        | $< "ab" $ "ab_star" >$ >> ) ]]]%prods_assignment;
+         Valid_nonterminal_symbols := (""::"ab"::"ab_star"::nil)%string |}.
+
     Definition make_parse_of : forall (str : string)
-                                      (prods : productions),
+                                      (prods : productions Ascii.ascii),
                                  bool
-      := @brute_force_make_parse_of trivial_grammar.
+      := @brute_force_make_parse_of ab_star_grammar.
 
 
 
     Definition parse : string -> bool
-      := fun str => make_parse_of str trivial_grammar.
+      := fun str => make_parse_of str ab_star_grammar.
 
-    Time Compute parse "".
-    Check eq_refl : true = parse "".
-    Time Compute parse "a".
-    Check eq_refl : false = parse "a".
-    Time Compute parse "aa".
-    Check eq_refl : false = parse "aa".
-  End example_parse_empty_grammar.
-
-  Section examples.
-    Section ab_star.
-
-      Fixpoint production_of_string (s : string) : production
-        := match s with
-             | EmptyString => nil
-             | String.String ch s' => (Terminal ch)::production_of_string s'
-           end.
-
-      Coercion production_of_string : string >-> production.
-
-      Fixpoint list_to_productions {T} (default : T) (ls : list (string * T)) : string -> T
-        := match ls with
-             | nil => fun _ => default
-             | (str, t)::ls' => fun s => if string_dec str s
-                                         then t
-                                         else list_to_productions default ls' s
-           end.
-
-      Delimit Scope item_scope with item.
-      Bind Scope item_scope with item.
-      Delimit Scope production_scope with production.
-      Delimit Scope production_assignment_scope with prod_assignment.
-      Bind Scope production_scope with production.
-      Delimit Scope productions_scope with productions.
-      Delimit Scope productions_assignment_scope with prods_assignment.
-      Bind Scope productions_scope with productions.
-      Notation "n0 ::== r0" := ((n0 : string)%string, (r0 : productions)%productions) (at level 100) : production_assignment_scope.
-      Notation "[[[ x ;; .. ;; y ]]]" :=
-        (list_to_productions (nil::nil) (cons x%prod_assignment .. (cons y%prod_assignment nil) .. )) : productions_assignment_scope.
-
-      Local Open Scope string_scope.
-      Notation "<< x | .. | y >>" :=
-        (@cons production (x)%production .. (@cons production (y)%production nil) .. ) : productions_scope.
-
-        Notation "$< x $ .. $ y >$" := (cons (NonTerminal x) .. (cons (NonTerminal y) nil) .. ) : production_scope.
-
-        Definition ab_star_grammar : grammar :=
-          {| Start_symbol := "ab_star";
-             Lookup := [[[ ("" ::== (<< "" >>)) ;;
-                                                ("ab" ::== << "ab" >>) ;;
-                                                ("ab_star" ::== << $< "" >$
-                                                | $< "ab" $ "ab_star" >$ >> ) ]]]%prods_assignment;
-             Valid_nonterminal_symbols := (""::"ab"::"ab_star"::nil)%string |}.
-
-        Definition make_parse_of : forall (str : string)
-                                          (prods : productions),
-                                     bool
-          := @brute_force_make_parse_of ab_star_grammar.
-
-
-
-        Definition parse : string -> bool
-          := fun str => make_parse_of str ab_star_grammar.
-
-        Time Eval lazy in parse "".
-        Check eq_refl : parse "" = true.
-        Time Eval lazy in parse "a".
-        Check eq_refl : parse "a" = false.
-        Time Eval lazy in parse "ab".
-        Check eq_refl : parse "ab" = true.
-        Time Eval lazy in parse "aa".
-        Check eq_refl : parse "aa" = false.
-        Time Eval lazy in parse "ba".
-        Check eq_refl : parse "ba" = false.
-        Time Eval lazy in parse "aba".
-        Check eq_refl : parse "aba" = false.
-        Time Eval lazy in parse "abab".
-        Time Eval lazy in parse "ababab".
-        Check eq_refl : parse "ababab" = true.
-    (* For debugging: *)(*
+    Time Eval lazy in parse "".
+    Check eq_refl : parse "" = true.
+    Time Eval lazy in parse "a".
+    Check eq_refl : parse "a" = false.
+    Time Eval lazy in parse "ab".
+    Check eq_refl : parse "ab" = true.
+    Time Eval lazy in parse "aa".
+    Check eq_refl : parse "aa" = false.
+    Time Eval lazy in parse "ba".
+    Check eq_refl : parse "ba" = false.
+    Time Eval lazy in parse "aba".
+    Check eq_refl : parse "aba" = false.
+    Time Eval lazy in parse "abab".
+    Time Eval lazy in parse "ababab".
+    Check eq_refl : parse "ababab" = true.
+  (* For debugging: *)(*
   Goal True.
     pose proof (eq_refl (parse "abab")) as s.
     unfold parse in s.
@@ -366,7 +403,6 @@ Module Export RecursiveDescentBooleanParserWithStringListHelper.
     do_compute_in (lt_dec (Length string_stringlike "abab"%string) (Length string_stringlike "abab"%string)) s.
     change (if in_right then ?x else ?y) with y in s.
     cbv beta zeta delta [rdp_list_is_valid_productions] in s.
-                         *)
-    End ab_star.
-  End examples.
-End RecursiveDescentBooleanParserWithStringListHelper.
+                       *)
+  End ab_star.
+End examples.
