src/Parsers/ContextFreeGrammar.v
@@ -3,9 +3,13 @@ Require Import Coq.Strings.String Coq.Lists.List Coq.Program.Program.
 Require Export Parsers.StringLike.
 
 Set Implicit Arguments.
+Local Set Boolean Equality Schemes.
+Local Set Decidable Equality Schemes.
 
-Module ContextFreeGrammar (S : StringLike).
-  Import S.
+Delimit Scope string_like_scope with string_like.
+
+Section cfg.
+  Variable CharType : Type.
 
   Section definitions.
     (** An [item] is the basic building block of a context-free
@@ -32,6 +36,7 @@ Module ContextFreeGrammar (S : StringLike).
 
     (** A [grammar] consists of [productions] to match a string
         against, and a function mapping names to [productions]. *)
+    (** TODO(jgross): also include list of valid starting non-terminals, for convenience and notation *)
     (** TODO(jgross): look up notations for specifying these nicely *)
     Record grammar :=
       {
@@ -44,35 +49,35 @@ Module ContextFreeGrammar (S : StringLike).
   End definitions.
 
   Section parse.
+    Variable String : string_like CharType.
     Variable G : grammar.
     (** A parse of a string into [productions] is a [production] in
         that list, together with a list of substrings which cover the
         original string, each of which is a parse of the relevant
         component of the [production]. *)
-    Inductive parse_of : t -> productions -> Type :=
+    Inductive parse_of : String -> productions -> Type :=
     | ParseHead : forall str pat pats, parse_of_production str pat
                                        -> parse_of str (pat::pats)
     | ParseTail : forall str pat pats, parse_of str pats
                                        -> parse_of str (pat::pats)
-    with parse_of_production : t -> production -> Type :=
-    | ParseProductionNil : parse_of_production Empty nil
+    with parse_of_production : String -> production -> Type :=
+    | ParseProductionNil : parse_of_production (Empty _) nil
     | ParseProductionCons : forall str pat strs pats,
                            parse_of_item str pat
                            -> parse_of_production strs pats
                            -> parse_of_production (str ++ strs) (pat::pats)
-    with parse_of_item : t -> item -> Type :=
+    with parse_of_item : String -> item -> Type :=
     | ParseTerminal : forall x, parse_of_item [[ x ]]%string_like (Terminal x)
     | ParseNonTerminal : forall name str, parse_of str (Lookup G name)
                                           -> parse_of_item str (NonTerminal name).
 
     Definition ParseProductionSingleton str it (p : parse_of_item str it) : parse_of_production str [ it ].
     Proof.
-      rewrite <- (RightId str).
+      rewrite <- (RightId _ str).
       constructor; assumption || constructor.
     Defined.
 
-    Definition ParseProductionApp str1 str2 p1 p2
-               (pop1 : parse_of_production str1 p1) (pop2 : parse_of_production str2 p2)
+    Definition ParseProductionApp str1 str2 p1 p2 (pop1 : parse_of_production str1 p1) (pop2 : parse_of_production str2 p2)
     : parse_of_production (str1 ++ str2) (p1 ++ p2)%list.
     Proof.
       induction pop1; simpl.
@@ -92,16 +97,46 @@ Module ContextFreeGrammar (S : StringLike).
     Defined.
   End parse.
 
-  Definition parse_of_grammar (str : t) (G : grammar) :=
-    parse_of G str G.
+  Definition parse_of_grammar (String : string_like CharType) (str : String) (G : grammar) :=
+    parse_of String G str G.
+End cfg.
 
+Arguments parse_of _%type_scope _ _ _%string_like _.
+Arguments parse_of_item _%type_scope _ _ _%string_like _.
+Arguments parse_of_production _%type_scope _ _ _%string_like _.
+Arguments parse_of_grammar _%type_scope _ _%string_like _.
+
+Local Hint Extern 0 => match goal with H : S _ = 0 |- _ => destruct (NPeano.Nat.neq_succ_0 _ H) end.
+
+Definition string_stringlike : string_like Ascii.ascii.
+Proof.
+  refine {| String := string;
+            Singleton := fun x => String.String x EmptyString;
+            Empty := EmptyString;
+            Concat := append;
+            Length := String.length;
+            bool_eq x y := if string_dec x y then true else false |};
+  solve [ abstract (let x := fresh "x" in
+                    let IHx := fresh "IHx" in
+                    intro x; induction x as [|? ? IHx]; try reflexivity; simpl;
+                    intros;
+                    f_equal;
+                    auto)
+        | intros; split; congruence
+        | intros; edestruct string_dec; split; congruence ].
+Defined.
+
+Section examples.
   Section generic.
-    Definition trivial_grammar : grammar :=
+    Variable CharType : Type.
+    Variable String : string_like CharType.
+
+    Definition trivial_grammar : grammar CharType :=
       {| Start_symbol := "";
          Lookup := fun _ => nil::nil;
          Valid_nonterminal_symbols := ""%string::nil |}.
 
-    Definition trivial_grammar_parses_empty_string : parse_of_grammar S.Empty trivial_grammar.
+    Definition trivial_grammar_parses_empty_string : parse_of_grammar _ (Empty String) trivial_grammar.
     Proof.
       hnf.
       simpl.
@@ -109,4 +144,4 @@ Module ContextFreeGrammar (S : StringLike).
       constructor.
     Qed.
   End generic.
-End ContextFreeGrammar.
+End examples.
