src/Parsers/Specification.v
@@ -1,14 +1,9 @@
 (** * Definition of a [comp]-based specification of a CFG parser-recognizer *)
-Require Import Computation.Core Parsers.StringLike Parsers.ContextFreeGrammar.
+Require Import Computation.Core Parsers.ContextFreeGrammar.
 
 Set Implicit Arguments.
 
-Module ParserSpecification (S : StringLike).
-  Import S.
-  Module Import G0 := ContextFreeGrammar S.
-
-  Definition parser_spec
-             (G : grammar)
-  : t -> Comp bool
-    := fun str => { b : bool | b = true <-> inhabited (parse_of_grammar str G) }%comp.
-End ParserSpecification.
+Definition parser_spec CharType (String : string_like CharType)
+           (G : grammar CharType)
+: String -> Comp bool
+  := fun str => { b : bool | b = true <-> inhabited (parse_of_grammar String str G) }%comp.
